code/ecdsap256/Hacl.Impl.P256.MM.Exponent.fst
@@ -432,7 +432,6 @@ let montgomery_ladder_power #c a scalar result =
   pop_frame()  
 
 
-#reset-options " --z3rlimit 200"
 let exponent #c a result = 
   match c with 
   |P384 ->
@@ -442,51 +441,61 @@ let exponent #c a result =
     exponent_p256 a result
 
 
-
-unfold let sqPower_list (#c: curve) : list uint8 =
-  match c with 
-  |P256 -> 
-    [
+inline_for_extraction noextract
+let sqPower_list_p256 : list uint8 =
+  [
       u8 0;  u8 0;  u8 0;  u8 0;   u8 0;   u8 0;   u8 0;   u8 0;
       u8 0;  u8 0;  u8 0;  u8 64;  u8 0;   u8 0;   u8 0;   u8 0;
       u8 0;  u8 0;  u8 0;  u8 0;   u8 0;   u8 0;   u8 0;   u8 64;
       u8 0;  u8 0;  u8 0;  u8 192; u8 255; u8 255; u8 255; u8 63
-    ]
-  |P384 -> 
-    [
-      u8 255; u8 255; u8 255; u8 63;  u8 0;   u8 0;   u8 0;   u8 0;
-      u8 0  ; u8 0  ; u8 0;   u8 192; u8 255; u8 255; u8 255; u8 191;
+  ]
+
+
+inline_for_extraction noextract
+let sqPower_list_p384 : list uint8 =
+    [ 
+      u8 0;   u8 0;   u8 0;   u8 64;  u8 0;   u8 0;   u8 0;   u8 0; 
+      u8 0;   u8 0;   u8 0;   u8 192; u8 255; u8 255; u8 255; u8 191;
+      u8 255; u8 255; u8 255; u8 255; u8 255; u8 255; u8 255; u8 255; 
+      u8 255; u8 255; u8 255; u8 255; u8 255; u8 255; u8 255; u8 255; 
       u8 255; u8 255; u8 255; u8 255; u8 255; u8 255; u8 255; u8 255;
-      u8 255; u8 255; u8 255; u8 255; u8 255; u8 255; u8 255; u8 255;
-      u8 255; u8 255; u8 255; u8 255; u8 255; u8 255; u8 255; u8 255;
-      u8 255; u8 255; u8 255; u8 255; u8 255; u8 255; u8 255; u8 63    
-    ]
+      u8 255; u8 255; u8 255; u8 255; u8 255; u8 255; u8 255; u8 63
+   ]
+
+
+inline_for_extraction noextract
+let sqPower_list (#c: curve) : list uint8 = 
+  match c with 
+  |P256 -> sqPower_list_p256
+  |P384 -> sqPower_list_p384
 
 
 let sqPower_seq (#c: curve) : s: lseq uint8 (getScalarLenNat c)
-  {Lib.ByteSequence.nat_from_intseq_le s == 
-  (getPrime c + 1) / 4} =
+  {
+    Lib.ByteSequence.nat_from_intseq_le s == (getPrime c + 1) / 4 /\
+    Lib.ByteSequence.nat_from_intseq_le s < getPrime c
+  } =
   let open Lib.ByteSequence in 
   assert_norm (List.Tot.length (sqPower_list #P256) == 32);
   assert_norm (List.Tot.length (sqPower_list #P384) == 48);
   
   nat_from_intlist_seq_le 32 (sqPower_list #P256);
-  nat_from_intlist_seq_le 48 (sqPower_list #P384);
+  nat_from_intlist_seq_le 48 (sqPower_list #P384); 
   
   assert_norm (nat_from_intlist_le (sqPower_list #P256)  == (getPrime P256 + 1) / 4);
   assert_norm (nat_from_intlist_le (sqPower_list #P384)  == (getPrime P384 + 1) / 4);
+  
   of_list (sqPower_list #c)
-
-
 
 
 inline_for_extraction
 let sqPower_buffer_p256 : x: glbuffer uint8 (getScalarLen P256) {witnessed x sqPower_seq /\ recallable x} = 
-  createL_global (sqPower_list #P256)
+  createL_global sqPower_list_p256
+
 
 inline_for_extraction
 let sqPower_buffer_p384 : x: glbuffer uint8 (getScalarLen P384) {witnessed x sqPower_seq /\ recallable x} = 
-  createL_global (sqPower_list #P384)
+  createL_global sqPower_list_p384
 
 inline_for_extraction
 let sqPower_buffer (#c: curve): (x: glbuffer uint8 (getScalarLen c)) = 
@@ -496,5 +505,5 @@ let sqPower_buffer (#c: curve): (x: glbuffer uint8 (getScalarLen c)) =
 
 
 let square_root #c a result = 
-  recall_contents sqPower_buffer (sqPower_seq #c);
+  recall_contents (sqPower_buffer #c) (sqPower_seq #c);
   montgomery_ladder_power a sqPower_buffer result
