code/ecdsap256/Hacl.Impl.P256.MM.Exponent.fsti
@@ -15,16 +15,16 @@ open Spec.P256
 val exponent: #c: curve -> a: felem c -> result: felem c
   -> Stack unit
     (requires fun h -> 
-      live h a /\ live h result /\  as_nat c h a < getPrime c)
+      live h a /\ live h result /\ as_nat c h a < getPrime c)
     (ensures fun h0 _ h1 -> 
       let k = fromDomain_ #c (as_nat c h0 a) in 
       modifies (loc a |+| loc result) h0 h1 /\
       as_nat c h1 result = toDomain_ #c (pow k (getPrime c - 2) % getPrime c))
 
 val square_root: #c: curve -> a: felem c -> result: felem c -> Stack unit 
-  (requires fun h -> live h a /\ live h result /\ as_nat c h a < prime256)
+  (requires fun h -> live h a /\ live h result /\ as_nat c h a < getPrime c)
   (ensures fun h0 _ h1 -> modifies (loc a |+| loc result) h0 h1 /\
-    as_nat c h1 result < prime256 /\
+    as_nat c h1 result < getPrime c /\
     fromDomain_ #c (as_nat c h1 result) = sq_root_spec #c (fromDomain_ #c (as_nat c h0 a)) /\
     fromDomain_ #c (as_nat c h1 result) = pow (fromDomain_ #c (as_nat c h0 a)) ((getPrime c + 1) / 4) % getPrime c
   )
